lean4/ProofChecker/ProofChecker/Data/ICnf.lean
@@ -30,6 +30,9 @@ def mkPos (x : Var) : ILit :=
 def mkNeg (x : Var) : ILit :=
   ⟨-Int.ofNat x.val, by simp⟩
 
+def mk (x : Var) (p : Bool) : ILit :=
+  if p then mkPos x else mkNeg x
+
 def var (l : ILit) : Var :=
   ⟨Int.natAbs l.val, Int.natAbs_pos.mpr l.property⟩
 
@@ -55,6 +58,22 @@ theorem var_mkNeg (x : Var) : var (mkNeg x) = x := by
   apply Subtype.ext
   simp [var, mkNeg]
   rfl
+  
+@[simp]
+theorem var_mk (x : Var) (p : Bool) : var (mk x p) = x := by
+  dsimp [mk]; split <;> simp
+
+@[simp]
+theorem polarity_mkPos (x : Var) : polarity (mkPos x) = true := by
+  simp [polarity, mkPos]
+
+@[simp]
+theorem polarity_mkNeg (x : Var) : polarity (mkNeg x) = false := by
+  simp [polarity, mkNeg]
+
+@[simp]
+theorem polarity_mk (x : Var) (p : Bool) : polarity (mk x p) = p := by
+  dsimp [mk]; split <;> simp_all
 
 @[simp]
 theorem var_negate (l : ILit) : (-l).var = l.var := by
@@ -66,6 +85,7 @@ theorem polarity_eq {l₁ l₂ : ILit} :
     l₁.polarity = l₂.polarity ↔ ((0 : Int) < l₁.val ↔ (0 : Int) < l₂.val) := by
   simp [polarity]
 
+@[simp]
 theorem polarity_negate (l : ILit) : (-l).polarity = !l.polarity := by
   rw [Bool.eq_bnot_to_not_eq, polarity_eq]
   intro hEq
@@ -88,6 +108,14 @@ theorem ext {l₁ l₂ : ILit} : l₁.var = l₂.var → l₁.polarity = l₂.po
     have : l₂ = 0 := Int.eq_zero_of_lt_neg_iff_lt l₂ h₂
     simp [this, h]
 
+@[simp]
+theorem eta (l : ILit) : mk l.var l.polarity = l := by
+  apply ext <;> simp
+
+@[simp]
+theorem eta_neg (l : ILit) : mk l.var (!l.polarity) = -l := by
+  apply ext <;> simp
+
 def toPropForm (l : ILit) : PropForm Var :=
   if l.polarity then .var l.var else .neg (.var l.var)
 
@@ -105,10 +133,23 @@ theorem satisfies_iff {τ : PropAssignment Var} {l : ILit} :
     τ ⊨ l.toPropTerm ↔ τ l.var = l.polarity := by
   dsimp [toPropTerm, var, polarity]
   aesop
+  
+theorem satisfies_neg {τ : PropAssignment Var} {l : ILit} :
+    τ ⊨ (-l).toPropTerm ↔ τ ⊭ l.toPropTerm := by
+  simp [satisfies_iff]
 
 theorem satisfies_set [DecidableEq ν] (τ : PropAssignment Var) (l : ILit) :
     τ.set l.var l.polarity ⊨ l.toPropTerm := by
   simp [satisfies_iff, τ.set_get]
+
+theorem eq_of_flip {τ : PropAssignment Var} {l : ILit} {x : Var} {p : Bool} :
+    τ ⊭ l.toPropTerm → τ.set x p ⊨ l.toPropTerm → l = mk x p := by
+  simp only [satisfies_iff]
+  intro h hSet
+  by_cases hEq : x = var l
+  . rw [hEq, τ.set_get] at hSet
+    simp [*]
+  . exfalso; exact h (τ.set_get_of_ne p hEq ▸ hSet)
 
 end ILit
 
@@ -129,15 +170,59 @@ instance : ToString IClause where
 
 /-! Theorems about `IClause` -/
 
-def toPropTerm : IClause → PropTerm Var :=
-  Array.foldr (init := ⊥) (fun l φ => l.toPropTerm ⊔ φ)
+def toPropTerm (C : IClause) : PropTerm Var :=
+  C.data.foldr (init := ⊥) (fun l φ => l.toPropTerm ⊔ φ)
   
 open PropTerm
 
 theorem satisfies_iff {τ : PropAssignment Var} {C : IClause} :
     τ ⊨ C.toPropTerm ↔ ∃ l ∈ C.data, τ ⊨ l.toPropTerm := by
-  rw [toPropTerm, Array.foldr_eq_foldr_data]
+  rw [toPropTerm]
   induction C.data <;> simp_all
+  
+theorem tautology_iff (C : IClause) :
+    C.toPropTerm = ⊤ ↔ ∃ l₁ ∈ C.data, ∃ l₂ ∈ C.data, l₁ = -l₂ := by
+  refine ⟨?mp, ?mpr⟩
+  case mp =>
+    refine not_imp_not.mp ?_
+    simp only [not_exists, not_and]
+    unfold toPropTerm -- :( have to do it because no induction principle for arrays
+    induction C.data with
+    | nil => simp
+    | cons l₀ ls ih =>
+      -- crazy list-array induction boilerplate
+      have : ls.foldr (init := ⊥) (fun l φ => l.toPropTerm ⊔ φ) = toPropTerm ls.toArray := by
+        simp [toPropTerm]
+      simp only [List.foldr_cons, this] at *
+      -- end boilerplate
+      intro hCompl hEq
+      specialize ih fun l₁ h₁ l₂ h₂ => hCompl l₁ (by simp [h₁]) l₂ (by simp [h₂])
+      simp only [PropTerm.eq_top_iff, satisfies_disj, not_forall] at hEq ih
+      have ⟨τ₀, h₀⟩ := ih
+      have := hEq τ₀
+      have : τ₀ ⊨ l₀.toPropTerm := by tauto
+      let τ₁ := τ₀.set l₀.var !l₀.polarity
+      have : τ₁ ⊭ l₀.toPropTerm := by simp [ILit.satisfies_iff]
+      have : τ₁ ⊭ toPropTerm ls.toArray := fun h => by
+        have ⟨lₛ, hₛ, hτ⟩ := satisfies_iff.mp h
+        simp only [satisfies_iff, not_exists, not_and] at h₀
+        have : τ₀ ⊭ lₛ.toPropTerm := h₀ lₛ hₛ
+        have : lₛ = ILit.mk l₀.var !l₀.polarity := ILit.eq_of_flip this hτ
+        have : lₛ = -l₀ := by simp [this]
+        simp at hₛ
+        apply hCompl lₛ (List.mem_cons_of_mem _ hₛ) l₀ (List.mem_cons_self _ _) this
+      have := hEq τ₁
+      tauto
+  case mpr =>
+    intro ⟨l₁, h₁, l₂, h₂, hEq⟩
+    ext τ
+    rw [satisfies_iff]
+    by_cases hτ : τ ⊨ l₂.toPropTerm
+    . aesop
+    . have : τ ⊨ l₁.toPropTerm := by
+        rw [hEq, ILit.satisfies_neg]
+        assumption
+      tauto
 
 end IClause
 
@@ -147,22 +232,22 @@ abbrev ICnf := Array IClause
 
 namespace ICnf
 
-def vars (C : ICnf) : HashSet Var :=
-  C.foldr (init := .empty Var) fun C acc => acc.union C.vars
+def vars (φ : ICnf) : HashSet Var :=
+  φ.foldr (init := .empty Var) fun C acc => acc.union C.vars
 
 instance : ToString ICnf where
   toString C := s!"{String.intercalate " ∧ " (C.map toString).toList}"
 
 /-! Theorems about `ICnf` -/
 
-def toPropTerm : ICnf → PropTerm Var :=
-  Array.foldr (init := ⊤) (fun l φ => l.toPropTerm ⊓ φ)
-  
+def toPropTerm (φ : ICnf) : PropTerm Var :=
+  φ.data.foldr (init := ⊤) (fun l φ => l.toPropTerm ⊓ φ)
+
 open PropTerm
   
 theorem satisfies_iff {τ : PropAssignment Var} {φ : ICnf} :
     τ ⊨ φ.toPropTerm ↔ ∀ C ∈ φ.data, τ ⊨ C.toPropTerm := by
-  rw [toPropTerm, Array.foldr_eq_foldr_data]
+  rw [toPropTerm]
   induction φ.data <;> simp_all
 
 end ICnf
@@ -179,6 +264,32 @@ namespace PartPropAssignment
 /-- Interpret the assignment (x ↦ ⊤, y ↦ ⊥) as x ∧ ¬y, for example. -/
 def toPropTerm (τ : PartPropAssignment) : PropTerm Var :=
   τ.fold (init := ⊤) fun acc x v => acc ⊓ if v then .var x else (.var x)ᶜ
+  
+open PropTerm
+  
+theorem satisfies_iff (τ : PartPropAssignment) (σ : PropAssignment Var) :
+    σ ⊨ τ.toPropTerm ↔ ∀ x p, τ.find? x = some p → σ x = p :=
+  ⟨mp, mpr⟩
+where
+  mp := fun h => by
+    intro x p? hFind
+    have ⟨φ, hφ⟩ := τ.fold_of_mapsTo_of_comm
+      (init := ⊤) (f := fun acc x v => acc ⊓ if v then PropTerm.var x else (PropTerm.var x)ᶜ)
+      hFind ?comm
+    case comm => 
+      intros
+      dsimp
+      ac_rfl
+    rw [toPropTerm, hφ] at h
+    aesop
+
+  mpr := fun h => by
+    apply HashMap.foldRecOn (hInit := satisfies_tr)
+    intro φ x p hφ hFind
+    rw [satisfies_conj]
+    refine ⟨hφ, ?_⟩
+    have := h _ _ hFind
+    split <;> simp [*]
 
 end PartPropAssignment
 
@@ -192,14 +303,63 @@ def reduce (C : IClause) (τ : PartPropAssignment) : Option IClause :=
     | some v => if v == l.polarity then none else acc
     | none => some <| acc.push l
     
--- TODO: What's the `reduce` theorem?
+-- theorem reduce_thm (C C' : IClause) (τ : PartPropAssignment) :
+--   reduce C τ = some C' → C.toPropTerm ⊓ τ.toPropTerm ≤ C'.toPropTerm := by
 
-/-- When `C` is not a tautology, return the smallest assignment falsifying it. When it is, return
-an undetermined assignment. -/
+/-- When `C` is not a tautology, return the smallest assignment falsifying it. When it is not,
+return an undetermined assignment. -/
 def toFalsifyingAssignment (C : IClause) : PartPropAssignment :=
-  C.foldr (init := .empty) fun l acc => acc.insert l.var !l.polarity
+  C.foldl (init := .empty) fun acc l => acc.insert l.var !l.polarity
 
-theorem toPropTerm_toFalsifyingAssignment (C : IClause) :
+theorem toFalsifyingAssignment_characterization (C : IClause) : C.toPropTerm ≠ ⊤ →
+    (∀ i : Fin C.size, C.toFalsifyingAssignment.find? C[i].var = some !C[i].polarity) ∧
+    (∀ x p, C.toFalsifyingAssignment.find? x = some p → (ILit.mk x !p) ∈ C.data) := by
+  intro hTauto
+  have := C.foldl_induction
+    (motive := fun (sz : Nat) (τ : PartPropAssignment) =>
+      (∀ i : Fin C.size, i < sz → τ.find? C[i].var = some !C[i].polarity) ∧
+      (∀ x p, τ.find? x = some p → (ILit.mk x !p) ∈ C.data))
+    (init := .empty)
+    (f := fun acc l => acc.insert l.var !l.polarity)
+    (h0 := by simp)
+    (hf := by
+      intro sz τ ⟨ih₁, ih₂⟩
+      refine ⟨?step₁, ?step₂⟩
+      case step₁ =>
+        intro i hLt
+        cases Nat.lt_or_eq_of_le (Nat.le_of_lt_succ hLt) with
+        | inl h =>
+          by_cases hEq : C[sz].var = C[i].var
+          . have : C[sz].polarity = C[i].polarity := by
+              by_contra hPol
+              have : C[sz] = -C[i] := by
+                apply ILit.ext <;> simp_all
+              apply hTauto
+              rw [tautology_iff]
+              exact ⟨C[sz], Array.get_mem_data _ _, C[i], Array.get_mem_data _ _, this⟩
+            have : C[sz] = C[i] := ILit.ext hEq this
+            simp_all [HashMap.find?_insert]
+          . simp only [HashMap.find?_insert_of_ne _ _ (bne_iff_ne _ _ |>.mpr hEq), ih₁ i h]
+        | inr h =>
+          simp [h]
+          rw [HashMap.find?_insert _ _ LawfulBEq.rfl]
+      case step₂ =>
+        intro x p hFind
+        by_cases hEq : C[sz].var = x
+        . rw [← hEq, HashMap.find?_insert _ _ (LawfulBEq.rfl)] at hFind
+          injection hFind with hFind
+          rw [← hEq, ← hFind]
+          simp [Array.getElem_mem_data]
+        . rw [HashMap.find?_insert_of_ne _ _ (bne_iff_ne _ _|>.mpr hEq)] at hFind
+          apply ih₂ _ _ hFind)
+  dsimp [toFalsifyingAssignment]
+  exact ⟨fun i => this.left i i.isLt, this.right⟩
+
+theorem toFalsifyingAssignment_ext (C : IClause) : C.toPropTerm ≠ ⊤ →
+    l ∈ C.data ↔ (toFalsifyingAssignment C).find? l.var = some !l.polarity := by
+  sorry
+
+theorem toPropTerm_toFalsifyingAssignment (C : IClause) : C.toPropTerm ≠ ⊤ →
     C.toFalsifyingAssignment.toPropTerm = C.toPropTermᶜ := by
   sorry
 
